

Randomized Selection

Same start as for deterministic selection

SELECT(**A**,**i**,**n**)

```
1  if ( $n = 1$ )
2      then return  $A[1]$ 

3   $p = \text{MEDIAN}(A)$ 
4
5

6   $L = \{x \in A : x \leq p\}$ 
    $H = \{x \in A : x > p\}$ 

7  if  $i \leq |L|$ 
8      then SELECT( $L, i, |L|$ )
9      else SELECT( $H, i - |L|, |H|$ )
```

Choose pivot p randomly.

Randomized Selection

Same start as for deterministic selection

SELECT(**A**,**i**,**n**)

```
1  if ( $n = 1$ )
2      then return  $A[1]$ 

3   $p = A[\text{RANDOM}(1, n)]$ 
4
5

6   $L = \{x \in A : x \leq p\}$ 
    $H = \{x \in A : x > p\}$ 

7  if  $i \leq |L|$ 
8      then SELECT( $L, i, |L|$ )
9      else SELECT( $H, i - |L|, |H|$ )
```

Analysis

$$T(n) = \sum_{x=1}^n \Pr(\text{partition is } x \text{ smallest}) \cdot (\text{Running time when partition is } x \text{ smallest}) .$$

Using x and $n - x$ as an upper bound of the sizes of the two sides:

$$\begin{aligned} T(n) &\leq \sum_{x=1}^n \frac{1}{n} ((T(x) \text{ or } T(n-x)) + O(n)) \\ &\leq \sum_{x=1}^n \frac{1}{n} (T(\max\{x, n-x\}) + O(n)) \\ &\leq \left(\frac{1}{n}\right) \sum_{x=1}^n (T(\max\{x, n-x\})) + O(n) \end{aligned}$$

We now rewrite the max term. Notice that as x goes from 1 to n , the term $\max\{x, n-x\}$ takes on the values $n-1, n-2, n-3, \dots, n/2, n/2, n/2+1, n/2+2, \dots, n-1, n$. As an overestimate, we say that it takes all the values between $n/2$ and n twice. Thus we substitute and obtain

$$\begin{aligned} T(n) &\leq \left(\frac{2}{n} \sum_{x=0}^{n/2} T(n/2+x) \right) + O(n) \\ &= \frac{2}{n} T(n) + \left(\frac{2}{n} \sum_{x=0}^{n/2-1} T(n/2+x) \right) + O(n) \end{aligned}$$

Analysis

$$\begin{aligned} T(n) &\leq \left(\frac{2}{n} \sum_{x=0}^{n/2} T(n/2 + x) \right) + O(n) \\ &= \frac{2}{n} T(n) + \left(\frac{2}{n} \sum_{x=0}^{n/2-1} T(n/2 + x) \right) + O(n) \end{aligned}$$

We pulled out the $T(n)$ terms to emphasize them. We might be worried about having $T(n)$ on the right side of the equation, so we will bring it over the left-hand side and obtain

$$\left(1 - \frac{2}{n} \right) T(n) \leq \left(\frac{2}{n} \sum_{x=0}^{n/2-1} T(n/2 + x) \right) + O(n) .$$

We now multiply both sides of the inequality by $n/(n-2)$ to obtain:

$$T(n) \leq \left(\frac{2}{n-2} \sum_{x=0}^{n/2-1} T(n/2 + x) \right) + kn^2/(n-2) .$$

We have replaced the $O(n)$ by kn for some constant k before multiplying by $n/(n-2)$. We do this because we will need to for the proof by induction below.

We now have a recurrence in a nice form. $T(n)$ is on the left, and the right has terms of the form $T(x)$ for $x < n$. We can therefore “guess” that $T(n) = O(n)$ and try to prove it. More precisely, we will prove by induction that $T(n) \leq cn$ for some c . Since the recurrence is in the stated form, we can substitute in on the right hand side and obtain

Analysis

$$\begin{aligned} T(n) &\leq \left(\frac{2}{n-2} \sum_{x=0}^{n/2-1} T(n/2 + x) \right) + kn^2/(n-2) \\ &\leq \left(\frac{2}{n-2} \sum_{x=0}^{n/2-1} c(n/2 + x) \right) + kn^2/(n-2) \\ &= \left(\frac{2c}{n-2} \right) ((n/2)(n/2) + (n/2 - 1)(n/2)/2) + kn^2/(n-2) \\ &= \left(\frac{2c}{n-2} \right) (3n^2/8 - n/4) + kn^2/(n-2) \\ &= \left(\frac{c}{n-2} \right) (3n^2/4 - n/8) + kn^2/(n-2) \\ &= \frac{1}{n-2} ((3c/4 + k)n^2 - (c/8)n) \\ &= \frac{n}{n-2} ((3c/4 + k)n - (c/8)) \end{aligned}$$

Looking at this last term, we see that the leading $n/(n-2)$ is slightly larger than 1, so we can upper bound it by, say $7/6$ for $n \geq 14$ (there are many possible choices of upper bounds.) Our goal, remember, is to show that the term multiplying the n is at most c , and as we will see, this suffices.

So we get

$$T(n) \leq (7/6) ((3c/4 + k)n - (c/8)) .$$

Analysis

$$T(n) \leq (7/6) ((3c/4 + k)n - (c/8)) .$$

If the right hand side is at most cn we are done. Whether it is will depend on the relative values of c and k . Let's write the constraint we want

$$(7/6) ((3c/4 + k)n - (c/8)) \leq cn$$

and solve for c in terms of k . We get

$$(7c/8 + 7k/6 - c)n \leq 7c/48$$

or

$$(7k/6 - c/8)n \leq 7c/48.$$

Clearly, if $7k/6 - c/8 < 0$ this will hold. So we just choose c sufficiently larger than k , e.g. $c = 28k/3$ and we are done.